vale/code/lib/transformers/Vale.Transformers.Transform.fst
@@ -63,16 +63,12 @@ let lemma_codes_code (c:codes) (fuel:nat) (s:machine_state) :
     (ensures (machine_eval_codes c fuel s == machine_eval_code (Block c) fuel s)) = ()
 #pop-options
 
-assume val lemma_to_of : (s0:_) -> (sM:_) -> Lemma (state_to_S (state_of_S s0 sM) == {sM with ms_trace = []})
-
-let lemma_IR_equiv_states_to_equiv_states (vs0:vale_state) (s1 s2:machine_state) :
+let lemma_IR_equiv_states_to_equiv_states (s1 s2:machine_state) :
   Lemma
     (requires (
-        (same_domain vs0 s1) /\
         (IR.equiv_states s1 s2)))
     (ensures (
-        (same_domain vs0 s2) /\
-        (equiv_states (state_of_S vs0 s1) (state_of_S vs0 s2)))) = ()
+        (equiv_states (state_of_S s1) (state_of_S s2)))) = ()
 
 (* See fsti *)
 let lemma_reorder orig hint transformed va_s0 va_sM va_fM =
@@ -89,13 +85,11 @@ let lemma_reorder orig hint transformed va_s0 va_sM va_fM =
       lemma_codes_code tr va_fM (state_to_S va_s0);
       let Some s = machine_eval_code orig va_fM (state_to_S va_s0) in
       let Some s' = machine_eval_code transformed va_fM (state_to_S va_s0) in
-      assert (same_domain va_sM s);
-      lemma_IR_equiv_states_to_equiv_states va_sM s s';
+      lemma_IR_equiv_states_to_equiv_states s s';
       assert (eval_code orig va_s0 va_fM va_sM);
       assert ({s with ms_trace = []} == (state_to_S va_sM));
-      assert (same_domain va_sM s');
-      let va_sM' = state_of_S va_sM s' in
-      lemma_to_of va_sM s';
+      let va_sM' = state_of_S s' in
+      lemma_to_of s';
       assert (state_to_S va_sM' == {s' with ms_trace = []});
       assert (state_to_S va_sM == {s with ms_trace = []});
       assert (IR.equiv_states ({s with ms_trace = []}) ({s' with ms_trace = []}));
